@prefix dct: <http://purl.org/dc/terms/>.
@prefix document: <http://e-editiones.ch/ontology/document#>.
@prefix homotypic: <http://www.nie.org/ontology/homotypic#>.
@prefix stoff: <http://www.nie.org/ontology/standoff#>.
@prefix text: <http://www.e-editiones.ch/ontology/text#>.
@prefix owl: <http://www.w3.org/2002/07/owl#>.
@prefix rdfs: <http://www.w3.org/2000/01/rdf-schema#>.
@prefix xsd: <http://www.w3.org/2001/XMLSchema#>.

@prefix tln: <http://www.nie.org/ontology/nietzsche#>.

<http://www.nie.org/ontology/nietzsche>
	a owl:Ontology;
	dct:license <http://creativecommons.org/licenses/by/3.0/>;
	dct:title "An ontology about the collected late works of Friedrich Nietzsche"@en;
	dct:description """Formal description of specific concepts in the scientific study of Friedrich Nietzsches late work."""@en;
	dct:creator "Dominique Steinbach, tool coordinator/software developer, NIE-INE/digital edition of der späte Nietzsche, Basel University, Switzerland"@en;
	dct:contributor "Christian Steiner, software developer, digital edition of der späte Nietzsche, University of Basel, Switzerland"@en;
   dct:publisher "Basel University, Switzerland"@en.


tln:Page a owl:Class ;
    rdfs:subClassOf document:Page .

tln:hasImage a owl:ObjectProperty ;
    rdfs:label "relates a page to a image"@en ;
    rdfs:comment "relates a page to an image that has a textfield that specifies the area where the writing that constitutes the page can be found."@en ;
    rdfs:isDefinedBy <http://www.nie.org/ontology/nietzsche> ;
    rdfs:domain tln:Page ;
    rdfs:range tln:Image .

tln:inheritOverwritesWord a owl:ObjectProperty ;
   rdfs:subPropertyOf tln:overwritesWord;
   rdfs:label "word overwrites word (inherited from tln:wordHasCorrection)"@en ;
   rdfs:comment "The author has used this word in order to overwrite that word."@en ;
   rdfs:isDefinedBy <http://www.nie.org/ontology/nietzsche> ;
   owl:propertyChainAxiom  ( tln:wordHasCorrection tln:overwritesWord ).

tln:lineContinuesOn a owl:ObjectProperty ;
    rdfs:label "writing from subject line continues on object line"@en ;
    rdfs:comment "the writing that ends on subject line continues on object line"@en ;
    rdfs:isDefinedBy <http://www.nie.org/ontology/nietzsche> ;
    rdfs:domain tln:Line ;
    rdfs:range tln:Line .

tln:pageIsOnTextField a a owl:ObjectProperty ;
    rdfs:label "page is on text field"@en ;
    rdfs:comment "the writing that is referred to as subject can be found on object"@en ;
    rdfs:isDefinedBy <http://www.nie.org/ontology/nietzsche> ;
    rdfs:domain tln:Page ;
    rdfs:range tln:TextField .

tln:writingContinuesWithWord a owl:ObjectProperty ;
    rdfs:label "writing continues with next word"@en ;
    rdfs:isDefinedBy <http://www.nie.org/ontology/nietzsche> ;
    rdfs:domain tln:Word ;
    rdfs:range tln:Word .
